

# MATH 411: Week 4

Jacob Lockard

13 February 2026

## Problem 7.31

Consider the series

$$\sum_{n=0}^{\infty} \frac{(-1)^n}{\sqrt{n+1}}.$$

(a) Explain (briefly) why the series converges. (Does it converge absolutely?)

(b) If we take the product of the series with itself, then we have

$$c_n = (-1)^n \sum_{k=0}^{\infty} \frac{1}{\sqrt{(n-k+1)(k+1)}}$$

(you should double check this). Show that each term in this sum is greater than or equal to  $\frac{1}{\sqrt{n+1}}$ , and thus  $|c_n| \geq \sqrt{n+1}$ .

(c) Explain (briefly) why the previous part implies  $\sum c_n$  diverges.

Define the series  $\sum_{n=0}^{\infty} a_n$  by

$$a_n = \frac{(-1)^n}{\sqrt{n+1}}.$$

(a) We'll show that  $\sum a_n$  converges absolutely. We note that for any  $n \in \mathbb{N}_0$ ,

$$\lim_{n \rightarrow \infty} \frac{\frac{1}{\sqrt{n+1}}}{\frac{1}{\sqrt{n}}} = \lim_{n \rightarrow \infty} \sqrt{\frac{n+1}{n}} = \lim_{n \rightarrow \infty} \sqrt{1 + \frac{1}{n}} = 1.$$

Since the sequence  $\left\{ \frac{1}{n^{1/2}} \right\}$  is a convergent  $p$ -series, the limit comparison test ensures  $\left\{ \frac{1}{\sqrt{n+1}} \right\}$  also converges. Since

$$\left| \frac{(-1)^n}{\sqrt{n+1}} \right| = \frac{1}{\sqrt{n+1}},$$

we conclude that  $\sum a_n$  converges absolutely.

(b) We will show that we have  $|c_n| > \sqrt{n+1}$  for all  $n$ , where  $\sum_{n=0}^{\infty} c_n$  is the Cauchy product of  $\sum a_n$  with itself. By definition,

$$c_n = (-1)^n \sum_{k=0}^n \frac{1}{\sqrt{(n-k+1)(k+1)}}.$$

If  $n \in \mathbb{N}_0$  and  $0 \leq k \leq n$ , we have

$$\begin{aligned} k &\leq n \\ k \cdot k &\leq nk \\ -k^2 &\geq -nk \\ nk - k^2 + n + 1 &\geq n + 1 \\ (n - k + 1)(k + 1) &\geq n + 1 \\ \sqrt{(n - k + 1)(k + 1)} &\geq \sqrt{n + 1} \\ \frac{1}{\sqrt{(n - k + 1)(k + 1)}} &\geq \frac{1}{\sqrt{n + 1}}, \end{aligned}$$

where the last line is justified by the fact that the square root function is non-negative and that here its arguments are nonzero. Now we can say that for any  $n \in \mathbb{N}_0$ ,

$$\begin{aligned} \sum_{k=0}^n \frac{1}{\sqrt{(n - k + 1)(k + 1)}} &\geq \sum_{k=0}^n \frac{1}{\sqrt{n + 1}} \\ &\geq \frac{n + 1}{\sqrt{n + 1}} \\ &= \sqrt{n + 1}. \end{aligned}$$

So for any  $n \in \mathbb{N}_0$ , we have  $|c_n| \geq \sqrt{n+1}$ .

(c) We'll show that  $\sum c_n$  diverges. The series  $\sum_{n=0}^{\infty} \sqrt{n+1}$  diverges, since its terms are unbounded. The comparison test then ensures  $\sum c_n$  also diverges.

□

## Problem 7.32

Let  $c_n = \sum_{k=0}^n c_n$  (where  $c_n$  is defined as above). Prove that  $C_n = a_0 B_{n-1} + \cdots + a_n B_0$  where  $B_n = \sum_{k=0}^n b_n$ . Define  $\beta_n = B_n - B$  and  $A_n = \sum_{k=0}^n a_n$ . Explain why the following are true:

(a)  $\lim_{n \rightarrow \infty} \beta_n = 0$

(b) For all  $N \geq 0$ ,  $C_n = A_n B + a_0 \beta_n + a_1 \beta_{n-1} + \cdots + a_n \beta_0$

$$(c) \lim_{n \rightarrow \infty} A_n B = AB$$

Let  $\sum_{n=0}^{\infty} A_n$  be an absolutely convergent series with  $\sum_{n=0}^{\infty} a_n = A$ , and let  $\sum_{n=0}^{\infty} b_n$  be a convergent series with  $\sum_{n=0}^{\infty} b_n = B$ . For all  $n \geq 0$ , define  $c_n = \sum_{k=0}^n a_k b_{n-k}$ ,  $C_n = \sum_{k=0}^n c_k$ , and  $\beta_n = B_n - B$ .

Let  $n \geq 0$ . We'll show that  $C_n = a_0 B_n + a_1 B_{n-1} + \cdots + a_n B_0$  where  $B_n = \sum_{k=0}^n b_k$ . We have:

$$\begin{aligned} C_n &= \sum_{k=0}^n c_k \\ &= (a_0 b_0) + (a_0 b_1 + a_1 b_0) + \cdots + (a_0 b_n + a_1 b_{n-1} + \cdots + a_n b_0) \\ &= a_0(b_0 + b_1 + \cdots + b_n) + a_1(b_0 + b_1 + \cdots + b_{n-1}) + \cdots + a_n b_0 \\ &= a_0 B_n + a_1 B_{n-1} + \cdots + a_n B_0. \end{aligned}$$

(a) We'll show that

$$\lim_{n \rightarrow \infty} \beta_n = 0.$$

Since  $\sum b_n = B$ , we know  $\{B_n\} \rightarrow B$ , and thus  $\{B_n - B\} \rightarrow B - B = 0$ .

(b) Let  $n \geq 0$ . We'll show that

$$C_n = A_n B + a_0 \beta_n + a_1 \beta_{n-1} + \cdots + a_n \beta_0.$$

We have:

$$\begin{aligned} \sum_{k=0}^n a_k \beta_{n-k} &= \sum_{k=0}^n a_k (B_{n-k} - B) \\ &= \sum_{k=0}^n a_k B_{n-k} - \sum_{k=0}^n a_k B \\ &= \sum_{k=0}^n a_k B_{n-k} - A_n B. \end{aligned}$$

We conclude:

$$C_n = \sum_{k=0}^n a_k B_{n-k} = \sum_{k=0}^n a_k \beta_{n-k} + A_n B.$$

(c) We will show that

$$\lim_{n \rightarrow \infty} A_n B = AB.$$

Since  $\{A_n\} \rightarrow A$  and  $\{B\}_{n=0}^{\infty} \rightarrow B$ , Problem 5.13 ensures  $\{A_n B\} \rightarrow AB$ .